theories/RHLE.v
@@ -1,5 +1,6 @@
 Require Import
         Coq.Arith.Arith
+        Coq.Sets.Ensembles
         Coq.micromega.Psatz
         Coq.Program.Tactics.
 
@@ -130,6 +131,29 @@ Section RHLE.
       eapply IHi0; congruence.
   Qed.
 
+  Lemma vector_replace_nth_id {A} {k}:
+    forall (i : Fin.t k) (v : t A k),
+      replace v i (nth v i) = v.
+  Proof.
+    induction i;
+      intros; pattern v; eapply caseS'; eauto; intros.
+    simpl; eauto.
+    rewrite IHi; reflexivity.
+  Qed.
+
+  Lemma vector_nth_exists {A} {k} (P : A -> Fin.t k -> Prop):
+    (forall (i : Fin.t k), exists (a : A), P a i) ->
+    exists (v : t A k), forall (i : Fin.t k), P (Vector.nth v i) i.
+  Proof.
+    induction k; intros.
+    - eexists (nil _); intros; inversion i.
+    - specialize (IHk (fun a i => P a (Fin.FS i)) (fun i => H (Fin.FS i))); destruct IHk.
+      destruct (H Fin.F1).
+      eexists (Vector.cons _ x0 _ x).
+      intros.
+      pattern i; eapply Fin.caseS'; intros; eauto.
+  Qed.
+
   Theorem rhle_proof_sound Sigs Sigma ESigma
           (Cons_Env : Consistent_Env {| AllEnv := {| funSigs := Sigs; funSpecs := Sigma; funDefs := empty |}; funExSpecs := ESigma |})
     : forall P c1 c2 Q,
@@ -203,24 +227,177 @@ Section RHLE.
         rewrite H; eauto.
   Qed.
 
-  (* Definition rwp (Sigma : Env) c (Q : Assertion2) : Assertion2 :=
-    fun st1 st2 => exists st2' (exe : Sigma |- st2 =[ c ]=> st2'), Q st1 st2'. *)
+  Inductive RelProductive
+            (Sigma : ExEnv)
+    : Estate -> Eprogs -> Ensemble Estate -> Prop :=
+  | RelP_Finish : forall Est Ec,
+      (forall i, Vector.nth Ec i = CSkip)
+      -> RelProductive Sigma Est Ec (Singleton _ Est)
 
-        (* Need to adjust this proof to align with new semantics. *)
-  (*Theorem rhle_proof_complete Sigs Sigma : forall P c1 c2 Q,
-      {| funSigs := Sigs; funSpecs := Sigma; funDefs := empty |} |= {{P}} c1 ~# c2 {[Q]} ->
-      Sigma |- {{P}} c1 ~# c2 {[Q]}.
+    | RelP_SkipIntro : forall Est Q Ec Ec' i,
+      (forall i', i <> i' -> Vector.nth Ec i' = Vector.nth Ec' i') ->
+      Vector.nth Ec' i = CSeq (Vector.nth Ec i) CSkip ->
+      RelProductive Sigma Est Ec' Q ->
+      RelProductive Sigma Est Ec Q
+
+  | RelP_Step :
+      forall Est Q (R : Ensemble state) Ec Ec' i c1 c2,
+        (forall i', i <> i' -> Vector.nth Ec i' = Vector.nth Ec' i') ->
+        Vector.nth Ec i = CSeq c1 c2 ->
+        Vector.nth Ec' i = c2 ->
+        Productive Sigma c1 (nth Est i) R ->
+        (forall st,
+            R st ->
+            RelProductive Sigma (replace Est i st) Ec' Q) ->
+        RelProductive Sigma Est Ec Q
+
+  | RelP_Weaken :
+      forall Est Ec Q Q',
+        RelProductive Sigma Est Ec Q ->
+        Included _ Q Q' ->
+        RelProductive Sigma Est Ec Q'.
+
+  Theorem RelProductive_produces (Sigma : ExEnv)
+  : forall (Est : Estate)
+           (Ec : Eprogs)
+           (Q : Ensemble Estate),
+      RelProductive Sigma Est Ec Q ->
+      exists Est'
+             (exe : forall i, AllEnv |- (Vector.nth Est i) =[Vector.nth Ec i]=> (Vector.nth Est' i)),
+        Q Est'.
   Proof.
-    unfold rhle_triple.
-    intros P c1 c2 Q H.
-    apply RHE_SkipIntroL.
-    apply RHE_StepL with (@rwp {| funSigs := Sigs; funSpecs := Sigma; funDefs := empty |} c2 Q).
-    - intros st2. eapply hoare_proof_complete with (Sigs := Sigs); firstorder.
-    - apply RHE_SkipIntroR. eapply RHE_StepR. 2: constructor.
-      intros st1.
+    induction 1.
+    - exists Est.
+      assert (forall i, AllEnv |- (Vector.nth Est i) =[Vector.nth Ec i]=> (Vector.nth Est i))
+        as exe
+        by (intros; rewrite H; eauto).
+      eexists exe; econstructor.
+    - destruct IHRelProductive as [Est' [exe QEst] ].
+      assert (forall (i' : Fin.t m), AllEnv |- nth Est i' =[ nth Ec i' ]=> nth Est' i')
+        as exe'.
+      { intros; destruct (Fin.eq_dec i i'); subst.
+        + specialize (exe i'); rewrite H0 in exe.
+          inversion exe; subst.
+          inversion X0; subst; eauto.
+        + rewrite H; eauto.
+      }
+      eauto.
+    - eapply productive_com_produces in H2; destruct H2 as [st' [exe' R_st'] ].
+      destruct (H4 _ R_st') as [Est' [exes' Q_exes'] ].
+      eexists Est'.
+      assert (forall (i' : Fin.t m), AllEnv |- nth Est i' =[ nth Ec i' ]=> nth Est' i'); eauto.
+      { intros; destruct (Fin.eq_dec i i'); subst.
+        + rewrite H0.
+          econstructor; eauto.
+          specialize (exes' i'); rewrite vector_nth_replace in exes'; eauto.
+        + rewrite H; eauto.
+          specialize (exes' i'); rewrite vector_nth_replace' in exes'; eauto.
+      }
+    - destruct IHRelProductive as [Est' [exes' Q_exes'] ].
+      eexists Est', exes'.
+      eapply H0; eauto.
+  Qed.
 
-      (* apply ehoare_proof_complete with (Sigs := Sigs); firstorder. *)
-  Admitted. *)
+  Theorem productive_Env_produces (Sigma : ExEnv)
+      : forall (Est : Estate)
+               (Ec : Eprogs)
+               (Q : Ensemble Estate),
+      productive_Env Sigma ->
+      RelProductive {| AllEnv := {|
+                                  funSigs := funSigs;
+                                  funSpecs := funSpecs;
+                                  funDefs := empty |};
+                       funExSpecs := funExSpecs |} Est Ec Q ->
+      RelProductive Sigma Est Ec Q.
+  Proof.
+    induction 2; intros; try (solve [econstructor; eauto]).
+    eapply RelP_Step; eauto using productive_Env_produces.
+  Qed.
+
+  Theorem rhle_proof_RelProductive Sigs Sigma ESigma
+          (Cons_Env : Consistent_Env {| AllEnv := {| funSigs := Sigs; funSpecs := Sigma; funDefs := empty |}; funExSpecs := ESigma |})
+    : forall P Uc Ec Q,
+      rhle_proof Sigma ESigma P Uc Ec Q ->
+      forall (Ust Ust' : Ustate)
+             (Est : Estate),
+        (forall (i : Fin.t n),
+            {| funSigs := Sigs; funSpecs := Sigma; funDefs := empty |}
+            |- Vector.nth Ust i =[ Vector.nth Uc i ]=> Vector.nth Ust' i) ->
+        P Ust Est ->
+        RelProductive {| AllEnv := {| funSigs := Sigs; funSpecs := Sigma; funDefs := empty |}; funExSpecs := ESigma |} Est Ec (Q Ust').
+  Proof.
+    intros ? ? ? ? pf.
+    induction pf; intros Ust Ust' Est exe HP.
+    - assert (Ust' = Ust).
+      { revert H exe; clear.
+        unfold Ustate in *; revert Ust Ust'.
+        induction Uc.
+        - intro; pattern Ust; eapply VectorDef.case0.
+          intro; pattern Ust'; eapply VectorDef.case0.
+          eauto.
+        - intro; pattern Ust; eapply VectorDef.caseS'.
+          intros h0 t Ust'; pattern Ust'; eapply VectorDef.caseS'.
+          intros; f_equal.
+          + specialize (H Fin.F1); specialize (exe Fin.F1); simpl in *.
+            subst; inversion exe; eauto.
+          + eapply IHUc; intros; eauto.
+            eapply (fun i => H (Fin.FS i)).
+            eapply (fun i => exe (Fin.FS i)).
+      }
+      assert (forall (i : Fin.t m), ceval {| funSigs := Sigs; funSpecs := Sigma; funDefs := @empty funDef |}  (nth Ec i) (nth Est i) (nth Est i)).
+      { revert H0; clear.
+        intros.
+        rewrite H0.
+        econstructor.
+      }
+      eapply RelP_Weaken.
+      econstructor; eauto.
+      unfold Included, Ensembles.In; intros Est' Inc_Est'; inversion Inc_Est'; subst; eauto.
+    - eapply IHpf in HP; eauto.
+      intros.
+      destruct (Fin.eq_dec i i0); subst.
+      + rewrite H0; eauto.
+      + rewrite <- H by eauto.
+        eapply exe.
+    - eapply IHpf in HP; eauto.
+      econstructor; eauto.
+    - generalize (exe i); intros exe'.
+      rewrite H0 in exe'; inversion exe'; subst.
+      eapply IHpf with (Ust := (replace Ust i st')).
+      + intros; destruct (Fin.eq_dec i i0); subst.
+        * rewrite vector_nth_replace; eauto.
+        * rewrite vector_nth_replace', <- H; eauto.
+      + eapply (hoare_proof_sound _ _ _ _ _ (H2 Ust Est) _ _ X); eauto.
+    - assert (nth Est i = nth Est i /\ P Ust Est) as H3 by tauto.
+      eapply RelP_Step; eauto.
+      eapply @ehoare_proof_produces with (Sigma := {| AllEnv := {| funSigs := _ |} |});
+        cbv beta; eauto using productive_empty.
+      + simpl; eauto.
+      + simpl; intros; eauto.
+  Qed.
+
+  Theorem rhle_proof_link
+          {Sigma : ExEnv}
+    : forall (P : RelAssertion)
+             (Uc : Uprogs)
+             (Ec : Eprogs)
+             (Q : RelAssertion),
+      productive_Env Sigma ->
+      Consistent_Env Sigma ->
+      safe_Env (@AllEnv Sigma) ->
+      (forall i Ust Est, P Ust Est ->
+                       @Safe {| funSigs := @funSigs (@AllEnv Sigma);
+                                funSpecs := @funSpecs (@AllEnv Sigma);
+                                funDefs := empty |} (Vector.nth Uc i) (Vector.nth Ust i)) ->
+      rhle_proof (@funSpecs (@AllEnv Sigma)) funExSpecs P Uc Ec Q ->
+      Sigma |= {{P}} Uc ~# Ec {[Q]}.
+  Proof.
+    unfold rhle_triple; intros.
+    eapply (rhle_proof_RelProductive funSigs _ _ H0 _ _ _ _ H2) in H3;
+      eauto using safe_Env_refine.
+    eapply productive_Env_produces in H3; eauto.
+    eapply RelProductive_produces in H3; eauto.
+  Qed.
 
 End RHLE.
 
@@ -230,8 +407,6 @@ End RHLE.
 Proof.
   unfold not; intros.
   assert  *)
-
-
 
 Notation "Sigma |= {{ P }}  c1 ~# c2  {[ Q ]}" :=
   (rhle_triple Sigma P c1 c2 Q) (at level 90, c1 at next level, c2 at next level)
